Foundation/Modal/Kripke/Logic/GrzPoint3.lean
@@ -23,7 +23,7 @@ variable {F : Frame}
 
 protected class Frame.IsFiniteGrzPoint3 (F : Frame) extends F.IsFinite, F.IsPartialOrder, F.IsPiecewiseStronglyConnected where
 
-abbrev FrameClass.finite_connected_partial_order : FrameClass := { F | F.IsFiniteGrzPoint3  }
+abbrev FrameClass.finite_GrzPoint3 : FrameClass := { F | F.IsFiniteGrzPoint3  }
 
 instance [F.IsFiniteGrzPoint3] : F.IsFiniteGrzPoint2 where
 
@@ -32,19 +32,19 @@ end Kripke
 
 namespace Logic.GrzPoint3.Kripke
 
-instance finite_sound : Sound Logic.GrzPoint3 FrameClass.finite_connected_partial_order := instSound_of_validates_axioms $ by
+instance finite_sound : Sound Hilbert.GrzPoint3 FrameClass.finite_GrzPoint3 := instSound_of_validates_axioms $ by
   apply FrameClass.Validates.withAxiomK;
   rintro F ⟨_, _, _⟩ _ (rfl | rfl);
   . exact validate_AxiomGrz_of_finite_strict_preorder;
   . exact validate_axiomPoint3_of_isPiecewiseStronglyConnected;
 
-instance : Entailment.Consistent Logic.GrzPoint3 :=
-  consistent_of_sound_frameclass FrameClass.finite_connected_partial_order $ by
+instance : Entailment.Consistent Hilbert.GrzPoint3 :=
+  consistent_of_sound_frameclass FrameClass.finite_GrzPoint3 $ by
     use whitepoint;
     constructor;
 
-instance finite_complete : Complete Logic.GrzPoint3 FrameClass.finite_connected_partial_order :=
-  Grz.Kripke.complete_of_mem_miniCanonicalFrame FrameClass.finite_connected_partial_order $ by
+instance finite_complete : Complete Hilbert.GrzPoint3 FrameClass.finite_GrzPoint3 :=
+  Hilbert.Grz.Kripke.complete_of_mem_miniCanonicalFrame FrameClass.finite_GrzPoint3 $ by
     sorry;
     /-
     intro φ;
@@ -84,23 +84,20 @@ open Formula
 open Entailment
 open Kripke
 
-lemma GrzPoint3.Kripke.finite_connected_partial_order : Logic.GrzPoint3 = FrameClass.finite_connected_partial_order.logic := eq_hilbert_logic_frameClass_logic
+lemma GrzPoint3.Kripke.finite_connected_partial_order : Modal.GrzPoint3 = FrameClass.finite_GrzPoint3.logic := eq_hilbert_logic_frameClass_logic
 
-theorem GrzPoint3.proper_extension_of_GrzPoint2: Logic.GrzPoint2 ⪱ Logic.GrzPoint3 := by
+theorem GrzPoint3.proper_extension_of_GrzPoint2: Hilbert.GrzPoint2 ⪱ Hilbert.GrzPoint3 := by
   constructor;
-  . apply Entailment.weakerThan_iff.mpr;
-    suffices ∀ φ, FrameClass.finite_GrzPoint2 ⊧ φ → FrameClass.finite_connected_partial_order ⊧ φ by
-      simpa [GrzPoint2.Kripke.finite_confluent_partial_order, GrzPoint3.Kripke.finite_connected_partial_order];
-    rintro φ hφ F hF;
-    apply hφ;
+  . apply Hilbert.Kripke.weakerThan_of_subset_frameClass FrameClass.finite_GrzPoint2 FrameClass.finite_GrzPoint3;
+    intro F hF;
     simp_all only [Set.mem_setOf_eq];
     infer_instance;
   . apply Entailment.not_weakerThan_iff.mpr;
-    suffices ∃ φ, Logic.GrzPoint3 ⊢! φ ∧ ¬FrameClass.finite_GrzPoint2 ⊧ φ by simpa [GrzPoint2.Kripke.finite_confluent_partial_order];
     use Axioms.Point3 (.atom 0) (.atom 1);
     constructor;
     . simp;
-    . apply Kripke.not_validOnFrameClass_of_exists_model_world;
+    . apply Sound.not_provable_of_countermodel (𝓜 := Kripke.FrameClass.finite_GrzPoint2);
+      apply Kripke.not_validOnFrameClass_of_exists_model_world;
       let F : Frame := ⟨Fin 4, λ x y => x = 0 ∨ x = y ∨ y = 3⟩;
       let M : Model := ⟨
         F,
@@ -141,16 +138,16 @@ theorem GrzPoint3.proper_extension_of_GrzPoint2: Logic.GrzPoint2 ⪱ Logic.GrzPo
             . tauto;
             . simp [M, Semantics.Realize, Satisfies, Frame.Rel', F];
 
-instance : Logic.S4Point3 ⪱ Logic.GrzPoint3 := by
+instance : Hilbert.S4Point3 ⪱ Hilbert.GrzPoint3 := by
   constructor;
   . apply Hilbert.Normal.weakerThan_of_provable_axioms;
     rintro _ (rfl | rfl | rfl | rfl) <;> simp;
   . apply Entailment.not_weakerThan_iff.mpr;
-    suffices ∃ φ, Logic.GrzPoint3 ⊢! φ ∧ ¬FrameClass.finite_S4Point3 ⊧ φ by simpa [S4Point3.Kripke.finite_connected_preorder];
     use Axioms.Grz (.atom 0);
     constructor;
     . simp;
-    . apply Kripke.not_validOnFrameClass_of_exists_model_world;
+    . apply Sound.not_provable_of_countermodel (𝓜 := Kripke.FrameClass.S4Point3);
+      apply Kripke.not_validOnFrameClass_of_exists_model_world;
       use ⟨⟨Fin 2, λ x y => True⟩, λ w _ => w = 1⟩, 0;
       constructor;
       . exact {
