Foundation/Modal/Kripke/Logic/S4Point2McK.lean
@@ -12,16 +12,16 @@ namespace Kripke
 
 variable {F : Kripke.Frame}
 
-class Frame.IsS4Point2McK (F : Kripke.Frame) extends F.IsReflexive, F.IsTransitive, F.SatisfiesMcKinseyCondition, F.IsPiecewiseStronglyConvergent where
+protected class Frame.IsS4Point2McK (F : Kripke.Frame) extends F.IsReflexive, F.IsTransitive, F.SatisfiesMcKinseyCondition, F.IsPiecewiseStronglyConvergent where
 
-abbrev FrameClass.preorder_confluent_mckinsey : FrameClass := { F | F.IsS4Point2McK }
+protected abbrev FrameClass.S4Point2McK : FrameClass := { F | F.IsS4Point2McK }
 
 end Kripke
 
 
-namespace Logic.S4Point2McK.Kripke
+namespace Hilbert.S4Point2McK.Kripke
 
-instance : Sound (Hilbert.S4Point2McK) Kripke.FrameClass.preorder_confluent_mckinsey := instSound_of_validates_axioms $ by
+instance : Sound (Hilbert.S4Point2McK) FrameClass.S4Point2McK := instSound_of_validates_axioms $ by
   apply FrameClass.Validates.withAxiomK;
   rintro F ⟨_⟩ _ (rfl | rfl | rfl | rfl);
   . exact validate_AxiomT_of_reflexive;
@@ -29,26 +29,26 @@ instance : Sound (Hilbert.S4Point2McK) Kripke.FrameClass.preorder_confluent_mcki
   . exact validate_axiomMcK_of_satisfiesMcKinseyCondition;
   . exact validate_AxiomPoint2_of_confluent;
 
-instance : Entailment.Consistent Logic.S4Point2McK :=
-  consistent_of_sound_frameclass FrameClass.preorder_confluent_mckinsey $ by
+instance : Entailment.Consistent Hilbert.S4Point2McK :=
+  consistent_of_sound_frameclass FrameClass.S4Point2McK $ by
     use whitepoint;
     constructor;
 
-instance : Canonical (Hilbert.S4Point2McK) Kripke.FrameClass.preorder_confluent_mckinsey := ⟨by constructor⟩
+instance : Canonical (Hilbert.S4Point2McK) FrameClass.S4Point2McK := ⟨by constructor⟩
 
-instance : Complete (Hilbert.S4Point2McK) Kripke.FrameClass.preorder_confluent_mckinsey := inferInstance
+instance : Complete (Hilbert.S4Point2McK) FrameClass.S4Point2McK := inferInstance
 
-lemma preorder_confluent_mckinsey : Logic.S4Point2McK = FrameClass.preorder_confluent_mckinsey.logic := eq_hilbert_logic_frameClass_logic
+lemma preorder_confluent_mckinsey : Modal.S4Point2McK = FrameClass.S4Point2McK.logic := eq_hilbert_logic_frameClass_logic
 
-instance : Logic.S4McK ⪱ Logic.S4Point2McK := by
+instance : Hilbert.S4McK ⪱ Hilbert.S4Point2McK := by
   constructor;
   . apply Hilbert.Normal.weakerThan_of_subset_axioms; intro φ; aesop;
   . apply Entailment.not_weakerThan_iff.mpr;
-    suffices ∃ φ, Logic.S4Point2McK ⊢! φ ∧ ¬Kripke.FrameClass.S4McK ⊧ φ by simpa [S4McK.Kripke.preorder_mckinsey];
     use (Axioms.Point2 (.atom 0));
     constructor;
     . simp;
-    . apply Kripke.not_validOnFrameClass_of_exists_model_world;
+    . apply Sound.not_provable_of_countermodel (𝓜 := Kripke.FrameClass.S4McK);
+      apply Kripke.not_validOnFrameClass_of_exists_model_world;
       let M : Model := ⟨⟨Fin 3, λ x y => x = 0 ∨ x = y⟩, λ w a => w = 1⟩;
       use M, 0;
       constructor
@@ -73,15 +73,15 @@ instance : Logic.S4McK ⪱ Logic.S4Point2McK := by
         . use 2;
           omega;
 
-instance : Logic.S4Point2 ⪱ Logic.S4Point2McK := by
+instance : Hilbert.S4Point2 ⪱ Hilbert.S4Point2McK := by
   constructor;
   . apply Hilbert.Normal.weakerThan_of_subset_axioms; intro φ; aesop;
   . apply Entailment.not_weakerThan_iff.mpr;
-    suffices ∃ φ, Logic.S4Point2McK ⊢! φ ∧ ¬FrameClass.S4Point2 ⊧ φ by simpa [S4Point2.Kripke.confluent_preorder];
     use (Axioms.McK (.atom 0))
     constructor;
     . simp;
-    . apply Kripke.not_validOnFrameClass_of_exists_model_world;
+    . apply Sound.not_provable_of_countermodel (𝓜 := Kripke.FrameClass.S4Point2);
+      apply Kripke.not_validOnFrameClass_of_exists_model_world;
       let M : Model := ⟨⟨Fin 2, λ x y => True⟩, λ w _ => w = 0⟩;
       use M, 0;
       constructor;
@@ -94,6 +94,6 @@ instance : Logic.S4Point2 ⪱ Logic.S4Point2McK := by
         use 1;
         trivial;
 
-end Logic.S4Point2McK.Kripke
+end Hilbert.S4Point2McK.Kripke
 
 end LO.Modal
