Foundation/Modal/Boxdot/K4_S4.lean
@@ -7,11 +7,8 @@ namespace LO.Modal
 
 open LO.Entailment LO.Entailment.FiniteContext LO.Modal.Entailment
 open Formula
-open Hilbert.Deduction
 
-namespace Logic
-
-lemma provable_boxdotTranslated_K4_of_provable_S4 : Logic.S4 ⊢! φ → Logic.K4 ⊢! φᵇ :=
+lemma provable_boxdotTranslated_K4_of_provable_S4 : Hilbert.S4 ⊢! φ → Hilbert.K4 ⊢! φᵇ :=
   Hilbert.of_provable_boxdotTranslated_axiomInstances $ by
     intro φ hp;
     rcases (by simpa using hp) with (⟨_, _, rfl⟩ | ⟨_, rfl⟩ | ⟨_, rfl⟩);
@@ -19,20 +16,18 @@ lemma provable_boxdotTranslated_K4_of_provable_S4 : Logic.S4 ⊢! φ → Logic.K
     . exact boxdot_axiomT!;
     . exact boxdot_axiomFour!
 
-lemma provable_S4_iff_boxdotTranslated : Logic.S4 ⊢! φ ⭤ φᵇ := by
+lemma provable_S4_iff_boxdotTranslated : Hilbert.S4 ⊢! φ ⭤ φᵇ := by
   induction φ with
   | hbox φ ihp => exact E!_trans (box_iff! ihp) iff_box_boxdot!;
   | himp φ ψ ihp ihq => exact ECC!_of_E!_of_E! ihp ihq;
   | _ => exact E!_id;
 
-lemma provable_S4_of_provable_boxdotTranslated_K4 (h : Logic.K4 ⊢! φᵇ) : Logic.S4 ⊢! φ := by
+lemma provable_S4_of_provable_boxdotTranslated_K4 (h : Hilbert.K4 ⊢! φᵇ) : Hilbert.S4 ⊢! φ := by
   exact (K!_right provable_S4_iff_boxdotTranslated) ⨀ (WeakerThan.pbl h);
 
-theorem iff_boxdotTranslatedK4_S4 : Logic.K4 ⊢! φᵇ ↔ Logic.S4 ⊢! φ := ⟨
+theorem iff_boxdotTranslatedK4_S4 : Hilbert.K4 ⊢! φᵇ ↔ Hilbert.S4 ⊢! φ := ⟨
   provable_S4_of_provable_boxdotTranslated_K4,
   provable_boxdotTranslated_K4_of_provable_S4
 ⟩
-
-end Logic
 
 end LO.Modal
