Foundation/Modal/Kripke/Logic/GL/Soundness.lean
@@ -28,12 +28,12 @@ end Kripke
 
 namespace Logic.GL.Kripke
 
-instance finite_sound : Sound Logic.GL FrameClass.finite_GL := instSound_of_validates_axioms $ by
+instance finite_sound : Sound Hilbert.GL FrameClass.finite_GL := instSound_of_validates_axioms $ by
   apply FrameClass.Validates.withAxiomK;
   rintro F ⟨_, _, _⟩ _ rfl;
   exact validate_AxiomL_of_trans_cwf;
 
-instance consistent : Entailment.Consistent Logic.GL :=
+instance consistent : Entailment.Consistent Hilbert.GL :=
   consistent_of_sound_frameclass FrameClass.finite_GL $ by
     use blackpoint;
     constructor;
