Foundation/Modal/Kripke/Logic/S5Grz.lean
@@ -9,22 +9,22 @@ open Formula
 open Kripke
 open Hilbert.Kripke
 
-instance : Logic.S5 ⪱ Logic.S5Grz := by
+instance : Hilbert.S5 ⪱ Hilbert.S5Grz := by
   constructor;
   . exact Hilbert.Normal.weakerThan_of_subset_axioms (by simp)
   . apply Entailment.not_weakerThan_iff.mpr;
     use Axioms.Grz (.atom 0);
     constructor;
     . simp;
-    . suffices ¬FrameClass.universal ⊧ (Axioms.Grz (.atom 0)) by simpa [S5.Kripke.universal];
+    . apply Sound.not_provable_of_countermodel (𝓜 := Kripke.FrameClass.universal);
       apply Kripke.not_validOnFrameClass_of_exists_model_world;
       use ⟨⟨Fin 2, λ x y => True⟩, λ w _ => w = 1⟩, 0;
       constructor;
-      . exact { universal := by tauto; };
+      . exact { universal := by tauto }
       . simp [Semantics.Realize, Satisfies];
         tauto;
 
-instance : Logic.Grz ⪱ Logic.S5Grz := by
+instance : Hilbert.Grz ⪱ Hilbert.S5Grz := by
   constructor;
   . apply Hilbert.Normal.weakerThan_of_provable_axioms;
     rintro _ (rfl | rfl | rfl) <;> simp;
@@ -32,7 +32,7 @@ instance : Logic.Grz ⪱ Logic.S5Grz := by
     use Axioms.Five (.atom 0)
     constructor;
     . simp;
-    . suffices ¬FrameClass.finite_Grz ⊧ Axioms.Five (.atom 0) by simpa [Grz.Kripke.finite_partial_order];
+    . apply Sound.not_provable_of_countermodel (𝓜 := Kripke.FrameClass.finite_Grz);
       apply Kripke.not_validOnFrameClass_of_exists_model_world;
       let M : Model := ⟨⟨Fin 2, λ x y => x ≤ y⟩, (λ w _ => w = 0)⟩;
       use M, 0;
@@ -49,16 +49,17 @@ instance : Logic.Grz ⪱ Logic.S5Grz := by
         . use 1;
           constructor <;> omega;
 
-instance : Logic.S4 ⪱ Logic.Triv := calc
-  Logic.S4 ⪱ Logic.S5    := by infer_instance
-  _        ⪱ Logic.S5Grz := by infer_instance
-  _        ≊ Logic.Triv  := by infer_instance
+instance : Hilbert.S4 ⪱ Hilbert.Triv := calc
+  Hilbert.S4 ⪱ Hilbert.S5    := by infer_instance
+  _          ⪱ Hilbert.S5Grz := by infer_instance
+  _          ≊ Hilbert.Triv  := by infer_instance
 
-instance : Sound Logic.S5Grz FrameClass.finite_Triv := by
-  suffices Sound Logic.Triv FrameClass.finite_Triv by
+/-
+instance : Sound Hilbert.S5Grz FrameClass.finite_Triv := by
+  suffices Sound Hilbert.Triv FrameClass.finite_Triv by
     convert this;
-    apply Logic.iff_equal_provable_equiv.mpr;
     infer_instance;
   infer_instance;
+-/
 
 end LO.Modal.Logic
